MemoryModel.fst: first implementation of preorder based concurrent memory model

fstar/MemoryModel.fst
@@ -2,32 +2,51 @@ module MemoryModel
 
 module U16 = FStar.UInt16
 module U8 = FStar.UInt8
+module Map = FStar.Map
+module P = FStar.Preorder
 
-assume val real_world_t:Type0
 
-assume val real_world_bind : real_world_t -> UInt8.t * real_world_t
+// type pointer = x:U16.t{U16.lt 0us x}
 
-noeq type state_t' = {
-     bytemap: U16.t -> U8.t;
-     real_world: real_world_t
+noeq type state_t = {
+     bytemap: Map.t U16.t U8.t;
   }
 
-assume val well_formed_state_t : state_t' -> prop
+assume val r0: P.preorder state_t
+assume val r1: P.preorder state_t
 
-let state_t = s:state_t'{well_formed_state_t s}
+let state_prop = state_t -> prop
+new_effect NONDET_STATE = STATE_h state_prop
 
-new_effect STATE = STATE_h state_t
-
-unfold let lift_div_state (a:Type) (wp:pure_wp a) (p:a -> state_t -> Type0) (h:state_t) =
+unfold let lift_div_state (a:Type) (wp:pure_wp a) (p:a -> state_prop -> Type0) (h:state_prop) =
   wp (fun a -> p a h)
 
-sub_effect DIV ~> STATE = lift_div_state
+sub_effect DIV ~> NONDET_STATE = lift_div_state
 
 effect ST (a:Type)
-  (pre:state_t -> Type0)
-  (post: (h:state_t -> a -> _:state_t{pre h} -> Type0)) =
-  STATE a (fun (p:(a -> state_t -> Type0)) (h:state_t) ->
+  (pre:state_prop -> Type0)
+  (post: (h:state_prop -> a -> _:state_prop{pre h} -> Type0)) =
+  NONDET_STATE a (fun (p:(a -> state_prop -> Type0)) (h:state_prop) ->
     pre h /\ (forall a h1. post h a h1 ==> p a h1))
 
 effect St (a:Type) = ST a (fun h -> True) (fun h0 r h1 -> True)
+
+assume val read0 (x:U16.t) :
+  ST U8.t
+    (fun p0 -> True)
+    (fun p0 v p1 -> 
+      let p (s:state_t) : prop = 
+        p0 s /\ Map.sel s.bytemap x == v
+      in
+      (exists s. p s) /\ (forall y. p1 y <==> (
+        exists x. r1 x y /\ p x
+      ))
+    )
+
+assume val write0 (key:U16.t) (v:U8.t) :
+  ST unit
+    (fun p0 -> forall s. p0 s ==> r1 s {bytemap = Map.upd s.bytemap key v})
+    (fun p0 _ p1 -> forall y. p1 y <==> (
+      exists x. p0 x /\ r1 {bytemap = Map.upd x.bytemap key v} y
+    ))
 
